pcuic/theories/PCUICGuardCondition.v
@@ -1,0 +1,101 @@
+(* Distributed under the terms of the MIT license. *)
+From MetaCoq.Template Require Import config utils.
+From MetaCoq.PCUIC Require Import PCUICAst PCUICAstUtils
+     PCUICEquality PCUICTyping PCUICNamelessDef PCUICSigmaCalculus
+     PCUICRenameDef PCUICInstDef.
+
+(* AXIOM postulate correctness of the guard condition checker *)
+
+Class GuardCheckerCorrect := 
+{
+  fix_guard_red1 Σ Γ mfix mfix' idx :
+      fix_guard Σ Γ mfix ->
+      red1 Σ Γ (tFix mfix idx) (tFix mfix' idx) ->
+      fix_guard Σ Γ mfix' ;
+
+  fix_guard_eq_term Σ Γ mfix mfix' idx :
+      fix_guard Σ Γ mfix ->
+      upto_names (tFix mfix idx) (tFix mfix' idx) ->
+      fix_guard Σ Γ mfix' ;
+
+  fix_guard_subst_instance {cf:checker_flags} Σ Γ mfix u univs :
+    consistent_instance_ext (Σ.1, univs) Σ.2 u ->
+    fix_guard Σ Γ mfix ->
+    fix_guard (Σ.1, univs) (subst_instance u Γ) (map (map_def (subst_instance u) (subst_instance u))
+                    mfix) ;
+
+  fix_guard_extends Σ Γ mfix Σ' : 
+    fix_guard Σ Γ mfix ->
+    extends Σ.1 Σ'.1 ->
+    fix_guard Σ' Γ mfix ;
+
+  fix_guard_context_cumulativity `{checker_flags} Σ Γ Γ' mfix :
+    All2_fold (cumul_decls Σ) Γ' Γ ->
+    fix_guard Σ Γ mfix ->
+    fix_guard Σ Γ' mfix ;
+
+  fix_guard_nl Σ Γ mfix :
+    fix_guard Σ Γ mfix -> fix_guard (nlg Σ) (nlctx Γ) (map (map_def_anon nl nl) mfix) ;
+  
+  fix_guard_inst `{checker_flags} Σ Γ Δ mfix σ :
+     Σ ;;; Γ ⊢ σ : Δ ->
+     let mfix' := map (map_def (inst σ) (inst (up (List.length mfix) σ))) mfix in
+     fix_guard Σ Δ mfix ->
+     fix_guard Σ Γ mfix' ;
+
+  fix_guard_rename P Σ Γ Δ mfix f :
+      urenaming P Γ Δ f ->
+      let mfix' := map (map_def (rename f) (rename (shiftn (List.length mfix) f))) mfix in
+      fix_guard Σ Δ mfix ->
+      fix_guard Σ Γ mfix' ;
+  
+  cofix_guard_red1 Σ Γ mfix mfix' idx :
+    cofix_guard Σ Γ mfix ->
+    red1 Σ Γ (tCoFix mfix idx) (tCoFix mfix' idx) ->
+    cofix_guard Σ Γ mfix' ;
+
+  cofix_guard_eq_term Σ Γ mfix mfix' idx :
+    cofix_guard Σ Γ mfix ->
+    upto_names (tCoFix mfix idx) (tCoFix mfix' idx) ->
+    cofix_guard Σ Γ mfix' ;
+
+  cofix_guard_lift Σ Γ Γ' Γ'' mfix :
+    let k' := (#|mfix| + #|Γ'|)%nat in
+    let mfix' := map (map_def (lift #|Γ''| #|Γ'|) (lift #|Γ''| k')) mfix in
+    cofix_guard Σ (Γ ,,, Γ') mfix ->
+    cofix_guard Σ (Γ ,,, Γ'' ,,, lift_context #|Γ''| 0 Γ') mfix' ;
+
+  cofix_guard_subst_instance {cf:checker_flags} Σ Γ mfix u univs :
+    consistent_instance_ext (Σ.1, univs) Σ.2 u ->
+    cofix_guard Σ Γ mfix ->
+    cofix_guard (Σ.1, univs) (subst_instance u Γ) (map (map_def (subst_instance u) (subst_instance u))
+                    mfix) ;
+  
+  cofix_guard_extends Σ Γ mfix Σ' : 
+    cofix_guard Σ Γ mfix ->
+    extends Σ.1 Σ'.1 ->
+    cofix_guard Σ' Γ mfix;
+
+  cofix_guard_context_cumulativity `{checker_flags} Σ Γ Γ' mfix :
+    All2_fold (cumul_decls Σ) Γ' Γ ->
+    cofix_guard Σ Γ mfix ->
+    cofix_guard Σ Γ' mfix ;
+
+  cofix_guard_nl Σ Γ mfix :
+    cofix_guard Σ Γ mfix -> cofix_guard (nlg Σ) (nlctx Γ) (map (map_def_anon nl nl) mfix) ;
+
+  cofix_guard_inst `{checker_flags} Σ Γ Δ mfix σ :
+    Σ ;;; Γ ⊢ σ : Δ ->
+    let mfix' := map (map_def (inst σ) (inst (up (List.length mfix) σ))) mfix in
+    cofix_guard Σ Δ mfix ->
+    cofix_guard Σ Γ mfix' ;
+
+  cofix_guard_rename P Σ Γ Δ mcofix f :
+      urenaming P Γ Δ f ->
+      let mcofix' := map (map_def (rename f) (rename (shiftn (List.length mcofix) f))) mcofix in
+      cofix_guard Σ Δ mcofix ->
+      cofix_guard Σ Γ mcofix' ;                                        
+}.
+
+Axiom guard_checking_correct : GuardCheckerCorrect.
+Existing Instance guard_checking_correct.
